HybridVerifVecs/KAT/HS_VC_KAT_ndfun.thy
@@ -1,109 +1,36 @@
 (*  Title:       Verification and refinement of hybrid systems in the relational KAT
-    Author:      Jonathan Julián Huerta y Munive, 2019
-    Maintainer:  Jonathan Julián Huerta y Munive <jjhuertaymunive1@sheffield.ac.uk>
+    Author:      Jonathan Julián Huerta y Munive, 2020
+    Maintainer:  Jonathan Julián Huerta y Munive <jonjulian23@gmail.com>
 *)
 
-section \<open> Verification and refinement of HS in the relational KAT \<close>
+subsection \<open>Verification of hybrid programs\<close>
 
 text \<open> We use our state transformers model to obtain verification and refinement components for 
-hybrid programs. We devise three methods for reasoning with evolution commands and their continuous 
-dynamics: providing flows, solutions or invariants. \<close>
+hybrid programs. We retake the three methods for reasoning with evolution commands and their 
+continuous dynamics: providing flows, solutions or invariants. \<close>
 
 theory HS_VC_KAT_ndfun
   imports 
-    "HS_VC_KAT"
     "../HS_ODEs"
-    "Transformer_Semantics.Kleisli_Quantale"
+    "../HS_VC_KAT"
+    "../HS_VC_KA_ndfun"
 
 begin
-
-subsection \<open> Store and Hoare triples \<close>
-
-type_synonym 'a pred = "'a \<Rightarrow> bool"
-
-\<comment> \<open>We start by deleting some conflicting notation.\<close>
-
-notation Abs_nd_fun ("_\<^sup>\<bullet>" [101] 100) 
-     and Rep_nd_fun ("_\<^sub>\<bullet>" [101] 100)
-
-declare Abs_nd_fun_inverse [simp]
-
-
-no_notation Archimedean_Field.ceiling ("\<lceil>_\<rceil>")
-        and Archimedean_Field.floor_ceiling_class.floor ("\<lfloor>_\<rfloor>")
-        and tau ("\<tau>")
-        and Relation.relcomp (infixl ";" 75)
-        and proto_near_quantale_class.bres (infixr "\<rightarrow>" 60)
-
-lemma nd_fun_ext: "(\<And>x. (f\<^sub>\<bullet>) x = (g\<^sub>\<bullet>) x) \<Longrightarrow> f = g"
-  apply(subgoal_tac "Rep_nd_fun f = Rep_nd_fun g")
-  using Rep_nd_fun_inject 
-   apply blast
-  by(rule ext, simp)
-
-lemma nd_fun_eq_iff: "(f = g) = (\<forall>x. (f\<^sub>\<bullet>) x = (g\<^sub>\<bullet>) x)"
-  by (auto simp: nd_fun_ext)
-
-instantiation nd_fun :: (type) kleene_algebra
-begin
-
-definition "0 = \<zeta>\<^sup>\<bullet>"
-
-definition "star_nd_fun f = qstar f" for f::"'a nd_fun"
-
-definition "f + g = ((f\<^sub>\<bullet>) \<squnion> (g\<^sub>\<bullet>))\<^sup>\<bullet>"
-
-thm sup_nd_fun_def sup_fun_def
-
-named_theorems nd_fun_aka "antidomain kleene algebra properties for nondeterministic functions."
-
-lemma nd_fun_plus_assoc[nd_fun_aka]: "x + y + z = x + (y + z)"
-  and nd_fun_plus_comm[nd_fun_aka]: "x + y = y + x"
-  and nd_fun_plus_idem[nd_fun_aka]: "x + x = x" for x::"'a nd_fun"
-  unfolding plus_nd_fun_def by (simp add: ksup_assoc, simp_all add: ksup_comm)
-
-lemma nd_fun_distr[nd_fun_aka]: "(x + y) \<cdot> z = x \<cdot> z + y \<cdot> z"
-  and nd_fun_distl[nd_fun_aka]: "x \<cdot> (y + z) = x \<cdot> y + x \<cdot> z" for x::"'a nd_fun"
-  unfolding plus_nd_fun_def times_nd_fun_def by (simp_all add: kcomp_distr kcomp_distl)
-
-lemma nd_fun_plus_zerol[nd_fun_aka]: "0 + x = x" 
-  and nd_fun_mult_zerol[nd_fun_aka]: "0 \<cdot> x = 0"
-  and nd_fun_mult_zeror[nd_fun_aka]: "x \<cdot> 0 = 0" for x::"'a nd_fun"
-  unfolding plus_nd_fun_def zero_nd_fun_def times_nd_fun_def by auto
-
-lemma nd_fun_leq[nd_fun_aka]: "(x \<le> y) = (x + y = y)"
-  and nd_fun_less[nd_fun_aka]: "(x < y) = (x + y = y \<and> x \<noteq> y)"
-  and nd_fun_leq_add[nd_fun_aka]: "z \<cdot> x \<le> z \<cdot> (x + y)" for x::"'a nd_fun"
-  unfolding less_eq_nd_fun_def less_nd_fun_def plus_nd_fun_def times_nd_fun_def sup_fun_def
-  by (unfold nd_fun_eq_iff le_fun_def, auto simp: kcomp_def)
-
-lemma nd_star_one[nd_fun_aka]: "1 + x \<cdot> x\<^sup>\<star> \<le> x\<^sup>\<star>"
-  and nd_star_unfoldl[nd_fun_aka]: "z + x \<cdot> y \<le> y \<Longrightarrow> x\<^sup>\<star> \<cdot> z \<le> y"
-  and nd_star_unfoldr[nd_fun_aka]: "z + y \<cdot> x \<le> y \<Longrightarrow> z \<cdot> x\<^sup>\<star> \<le> y" for x::"'a nd_fun"
-  unfolding plus_nd_fun_def star_nd_fun_def
-    apply(simp_all add: fun_star_inductl sup_nd_fun.rep_eq fun_star_inductr)
-  by (metis order_refl sup_nd_fun.rep_eq uwqlka.conway.dagger_unfoldl_eq)
-
-instance
-  apply intro_classes
-  using nd_fun_aka by simp_all
-
-end
 
 instantiation nd_fun :: (type) kat
 begin
 
 definition "n f = (\<lambda>x. if ((f\<^sub>\<bullet>) x = {}) then {x} else {})\<^sup>\<bullet>"
 
-lemma nd_fun_n_op_one[nd_fun_aka]: "n (n (1::'a nd_fun)) = 1"
-  and nd_fun_n_op_mult[nd_fun_aka]: "n (n (n x \<cdot> n y)) = n x \<cdot> n y"
-  and nd_fun_n_op_mult_comp[nd_fun_aka]: "n x \<cdot> n (n x) = 0" 
-  and nd_fun_n_op_de_morgan[nd_fun_aka]: "n (n (n x) \<cdot> n (n y)) = n x + n y" for x::"'a nd_fun"
+lemma nd_fun_n_op_one[nd_fun_ka]: "n (n (1::'a nd_fun)) = 1"
+  and nd_fun_n_op_mult[nd_fun_ka]: "n (n (n x \<cdot> n y)) = n x \<cdot> n y"
+  and nd_fun_n_op_mult_comp[nd_fun_ka]: "n x \<cdot> n (n x) = 0" 
+  and nd_fun_n_op_de_morgan[nd_fun_ka]: "n (n (n x) \<cdot> n (n y)) = n x + n y" for x::"'a nd_fun"
   unfolding n_op_nd_fun_def one_nd_fun_def times_nd_fun_def plus_nd_fun_def zero_nd_fun_def 
   by (auto simp: nd_fun_eq_iff kcomp_def)
 
 instance
-  by (intro_classes, auto simp: nd_fun_aka)
+  by (intro_classes, auto simp: nd_fun_ka)
 
 end
 
@@ -119,7 +46,18 @@ instance
 
 end
 
-\<comment> \<open>Canonical lifting from predicates to state transformers and its simplification rules\<close>
+
+subsubsection \<open> Regular programs\<close>
+
+text \<open> Lemmas for manipulation of predicates in the relational model \<close>
+
+type_synonym 'a pred = "'a \<Rightarrow> bool"
+
+no_notation Archimedean_Field.ceiling ("\<lceil>_\<rceil>")
+        and Archimedean_Field.floor_ceiling_class.floor ("\<lfloor>_\<rfloor>")
+        and tau ("\<tau>")
+        and Relation.relcomp (infixl ";" 75)
+        and proto_near_quantale_class.bres (infixr "\<rightarrow>" 60)
 
 definition p2ndf :: "'a pred \<Rightarrow> 'a nd_fun" ("(1\<lceil>_\<rceil>)")
   where "\<lceil>Q\<rceil> \<equiv> (\<lambda> x::'a. {s::'a. s = x \<and> Q s})\<^sup>\<bullet>"
@@ -134,82 +72,130 @@ lemma p2ndf_simps[simp]:
   unfolding p2ndf_def one_nd_fun_def less_eq_nd_fun_def times_nd_fun_def plus_nd_fun_def 
   by (auto simp: nd_fun_eq_iff kcomp_def le_fun_def n_op_nd_fun_def)
 
-\<comment> \<open> Meaning of the state-transformer Hoare triple \<close>
+text \<open> Lemmas for verification condition generation \<close>
 
-lemma ndfun_kat_H: "Hoare \<lceil>P\<rceil> X \<lceil>Q\<rceil> \<longleftrightarrow> (\<forall>s s'. P s \<longrightarrow> s' \<in> (X\<^sub>\<bullet>) s \<longrightarrow> Q s')"
+\<comment> \<open> Hoare Triples \<close>
+
+abbreviation ndfunHoare ("\<^bold>{_\<^bold>}_\<^bold>{_\<^bold>}") 
+  where "\<^bold>{P\<^bold>}X\<^bold>{Q\<^bold>} \<equiv> Hoare \<lceil>P\<rceil> X \<lceil>Q\<rceil>"
+
+lemma ndfun_kat_H: "\<^bold>{P\<^bold>} X \<^bold>{Q\<^bold>} \<longleftrightarrow> (\<forall>s s'. P s \<longrightarrow> s' \<in> (X\<^sub>\<bullet>) s \<longrightarrow> Q s')"
   unfolding Hoare_def p2ndf_def less_eq_nd_fun_def times_nd_fun_def kcomp_def 
   by (auto simp add: le_fun_def n_op_nd_fun_def)
 
-\<comment> \<open> Hoare triple for skip and a simp-rule \<close>
+\<comment> \<open> Skip \<close>
 
 abbreviation "skip \<equiv> (1::'a nd_fun)"
 
-lemma H_skip: "Hoare \<lceil>P\<rceil> skip \<lceil>P\<rceil>"
-  using H_skip by blast
-
-lemma sH_skip[simp]: "Hoare \<lceil>P\<rceil> skip \<lceil>Q\<rceil> \<longleftrightarrow> \<lceil>P\<rceil> \<le> \<lceil>Q\<rceil>"
+lemma sH_skip[simp]: "\<^bold>{P\<^bold>} skip \<^bold>{Q\<^bold>} \<longleftrightarrow> \<lceil>P\<rceil> \<le> \<lceil>Q\<rceil>"
   unfolding ndfun_kat_H by (simp add: one_nd_fun_def)
 
-\<comment> \<open> We introduce assignments and compute derive their rule of Hoare logic. \<close>
+lemma H_skip: "\<^bold>{P\<^bold>} skip \<^bold>{P\<^bold>}"
+  by simp
 
-definition vec_upd :: "('a^'b) \<Rightarrow> 'b \<Rightarrow> 'a \<Rightarrow> 'a^'b"
-  where "vec_upd s i a = (\<chi> j. ((($) s)(i := a)) j)"
+\<comment> \<open> Tests \<close>
+
+lemma sH_test[simp]: "\<^bold>{P\<^bold>} \<lceil>R\<rceil> \<^bold>{Q\<^bold>} = (\<forall>s. P s \<longrightarrow> R s \<longrightarrow> Q s)"
+  by (subst ndfun_kat_H, simp add: p2ndf_def)
+
+\<comment> \<open> Abort \<close>
+
+abbreviation "abort \<equiv> (0::'a nd_fun)"
+
+lemma sH_abort[simp]: "\<^bold>{P\<^bold>} abort \<^bold>{Q\<^bold>} \<longleftrightarrow> True"
+  unfolding ndfun_kat_H by (simp add: zero_nd_fun_def)
+
+lemma H_abort: "\<^bold>{P\<^bold>} abort \<^bold>{Q\<^bold>}"
+  by simp
+
+\<comment> \<open> Assignments \<close>
 
 definition assign :: "'b \<Rightarrow> ('a^'b \<Rightarrow> 'a) \<Rightarrow> ('a^'b) nd_fun" ("(2_ ::= _)" [70, 65] 61) 
   where "(x ::= e) = (\<lambda>s. {vec_upd s x (e s)})\<^sup>\<bullet>"
 
-lemma H_assign: "P = (\<lambda>s. Q (\<chi> j. ((($) s)(x := (e s))) j)) \<Longrightarrow> Hoare \<lceil>P\<rceil> (x ::= e) \<lceil>Q\<rceil>"
-  unfolding ndfun_kat_H assign_def vec_upd_def by force
-
-lemma sH_assign[simp]: "Hoare \<lceil>P\<rceil> (x ::= e) \<lceil>Q\<rceil> \<longleftrightarrow> (\<forall>s. P s \<longrightarrow> Q (\<chi> j. ((($) s)(x := (e s))) j))"
+lemma sH_assign[simp]: "\<^bold>{P\<^bold>} (x ::= e) \<^bold>{Q\<^bold>} \<longleftrightarrow> (\<forall>s. P s \<longrightarrow> Q (\<chi> j. ((($) s)(x := (e s))) j))"
   unfolding ndfun_kat_H vec_upd_def assign_def by (auto simp: fun_upd_def)
 
-\<comment> \<open> Next, the Hoare rule of the composition \<close>
+lemma H_assign: "P = (\<lambda>s. Q (\<chi> j. ((($) s)(x := (e s))) j)) \<Longrightarrow> \<^bold>{P\<^bold>} (x ::= e) \<^bold>{Q\<^bold>}"
+  by simp
+
+\<comment> \<open> Nondeterministic assignments \<close>
+
+definition nondet_assign :: "'b \<Rightarrow> ('a^'b) nd_fun" ("(2_ ::= ? )" [70] 61)
+    where "(x ::= ?) = (\<lambda>s. {vec_upd s x k|k. True})\<^sup>\<bullet>"
+
+lemma sH_nondet_assign[simp]: 
+  "\<^bold>{P\<^bold>} (x ::= ?) \<^bold>{Q\<^bold>} \<longleftrightarrow> (\<forall>s. P s \<longrightarrow> (\<forall>k. Q (\<chi> j. ((($) s)(x := k)) j)))"
+  unfolding ndfun_kat_H vec_upd_def nondet_assign_def by (auto simp: fun_upd_def)
+
+lemma H_nondet_assign: "\<^bold>{\<lambda>s. \<forall>k. P (\<chi> j. ((($) s)(x := k)) j)\<^bold>} (x ::= ?) \<^bold>{P\<^bold>}"
+  by simp
+
+\<comment> \<open> Sequential Composition \<close>
 
 abbreviation seq_seq :: "'a nd_fun \<Rightarrow> 'a nd_fun \<Rightarrow> 'a nd_fun" (infixl ";" 75)
   where "f ; g \<equiv> f \<cdot> g"
 
-lemma H_seq: "Hoare \<lceil>P\<rceil> X \<lceil>R\<rceil> \<Longrightarrow> Hoare \<lceil>R\<rceil> Y \<lceil>Q\<rceil> \<Longrightarrow> Hoare \<lceil>P\<rceil> (X ; Y) \<lceil>Q\<rceil>"
+lemma H_seq: "\<^bold>{P\<^bold>} X \<^bold>{R\<^bold>} \<Longrightarrow> \<^bold>{R\<^bold>} Y \<^bold>{Q\<^bold>} \<Longrightarrow> \<^bold>{P\<^bold>} X;Y \<^bold>{Q\<^bold>}"
   by (auto intro: H_seq)
 
-lemma sH_seq: "Hoare \<lceil>P\<rceil> (X ; Y) \<lceil>Q\<rceil> = Hoare \<lceil>P\<rceil> (X) \<lceil>\<lambda>s. \<forall>s'. s' \<in> (Y\<^sub>\<bullet>) s \<longrightarrow> Q s'\<rceil>"
+lemma sH_seq: "\<^bold>{P\<^bold>} X;Y \<^bold>{Q\<^bold>} = \<^bold>{P\<^bold>} X \<^bold>{\<lambda>s. \<forall>s'. s' \<in> (Y\<^sub>\<bullet>) s \<longrightarrow> Q s'\<^bold>}"
   unfolding ndfun_kat_H by (auto simp: times_nd_fun_def kcomp_def)
 
-\<comment> \<open> Rewriting the Hoare rule for the conditional statement \<close>
+lemma H_assignl: 
+  assumes "\<^bold>{K\<^bold>} X \<^bold>{Q\<^bold>}" 
+    and "\<forall>s. P s \<longrightarrow> K (vec_lambda ((($) s)(x := e s)))"
+  shows "\<^bold>{P\<^bold>} (x ::= e);X \<^bold>{Q\<^bold>}"
+  apply(rule H_seq, subst sH_assign)
+  using assms by auto
+
+\<comment> \<open> Nondeterministic Choice \<close>
+
+lemma sH_choice: "\<^bold>{P\<^bold>} X + Y \<^bold>{Q\<^bold>} \<longleftrightarrow> (\<^bold>{P\<^bold>} X \<^bold>{Q\<^bold>} \<and> \<^bold>{P\<^bold>} Y \<^bold>{Q\<^bold>})"
+  unfolding ndfun_kat_H by (auto simp: plus_nd_fun_def)
+
+lemma H_choice: "\<^bold>{P\<^bold>} X \<^bold>{Q\<^bold>} \<Longrightarrow> \<^bold>{P\<^bold>} Y \<^bold>{Q\<^bold>} \<Longrightarrow> \<^bold>{P\<^bold>} X + Y \<^bold>{Q\<^bold>}"
+  using H_choice .
+
+\<comment> \<open> Conditional Statement \<close>
 
 abbreviation cond_sugar :: "'a pred \<Rightarrow> 'a nd_fun \<Rightarrow> 'a nd_fun \<Rightarrow> 'a nd_fun" ("IF _ THEN _ ELSE _" [64,64] 63) 
   where "IF B THEN X ELSE Y \<equiv> kat_cond \<lceil>B\<rceil> X Y"
 
-lemma H_cond: "Hoare \<lceil>\<lambda>s. P s \<and> B s\<rceil> X \<lceil>Q\<rceil> \<Longrightarrow> Hoare \<lceil>\<lambda>s. P s \<and> \<not> B s\<rceil> Y \<lceil>Q\<rceil> \<Longrightarrow> 
-  Hoare \<lceil>P\<rceil> (IF B THEN X ELSE Y) \<lceil>Q\<rceil>"
-  by (rule H_cond, simp_all)
-
-lemma sH_cond[simp]: "Hoare \<lceil>P\<rceil> (IF B THEN X ELSE Y) \<lceil>Q\<rceil> \<longleftrightarrow> 
-  (Hoare \<lceil>\<lambda>s. P s \<and> B s\<rceil> X \<lceil>Q\<rceil> \<and> Hoare \<lceil>\<lambda>s. P s \<and> \<not> B s\<rceil> Y \<lceil>Q\<rceil>)"
+lemma sH_cond[simp]: 
+  "\<^bold>{P\<^bold>} (IF B THEN X ELSE Y) \<^bold>{Q\<^bold>} \<longleftrightarrow> (\<^bold>{\<lambda>s. P s \<and> B s\<^bold>} X \<^bold>{Q\<^bold>} \<and> \<^bold>{\<lambda>s. P s \<and> \<not> B s\<^bold>} Y \<^bold>{Q\<^bold>})"
   by (auto simp: H_cond_iff ndfun_kat_H)
 
-\<comment> \<open> Rewriting the Hoare rule for the while loop \<close>
+lemma H_cond: 
+  "\<^bold>{\<lambda>s. P s \<and> B s\<^bold>} X \<^bold>{Q\<^bold>} \<Longrightarrow> \<^bold>{\<lambda>s. P s \<and> \<not> B s\<^bold>} Y \<^bold>{Q\<^bold>} \<Longrightarrow> \<^bold>{P\<^bold>} (IF B THEN X ELSE Y) \<^bold>{Q\<^bold>}"
+  by simp
+
+\<comment> \<open> While Loop \<close>
 
 abbreviation while_inv_sugar :: "'a pred \<Rightarrow> 'a pred \<Rightarrow> 'a nd_fun \<Rightarrow> 'a nd_fun" ("WHILE _ INV _ DO _" [64,64,64] 63) 
   where "WHILE B INV I DO X \<equiv> kat_while_inv \<lceil>B\<rceil> \<lceil>I\<rceil> X"
 
-lemma sH_while_inv: "\<forall>s. P s \<longrightarrow> I s \<Longrightarrow> \<forall>s. I s \<and> \<not> B s \<longrightarrow> Q s \<Longrightarrow> Hoare \<lceil>\<lambda>s. I s \<and> B s\<rceil> X \<lceil>I\<rceil> 
-  \<Longrightarrow> Hoare \<lceil>P\<rceil> (WHILE B INV I DO X) \<lceil>Q\<rceil>"
+lemma sH_whileI: "\<forall>s. P s \<longrightarrow> I s \<Longrightarrow> \<forall>s. I s \<and> \<not> B s \<longrightarrow> Q s \<Longrightarrow> \<^bold>{\<lambda>s. I s \<and> B s\<^bold>} X \<^bold>{I\<^bold>} 
+  \<Longrightarrow> \<^bold>{P\<^bold>} (WHILE B INV I DO X) \<^bold>{Q\<^bold>}"
   by (rule H_while_inv, simp_all add: ndfun_kat_H)
 
-\<comment> \<open> Finally, we add a Hoare triple rule for finite iterations. \<close>
+lemma "\<^bold>{\<lambda>s. P s \<and> B s\<^bold>} X \<^bold>{\<lambda>s. P s\<^bold>} \<Longrightarrow> \<^bold>{P\<^bold>} (WHILE B INV I DO X) \<^bold>{\<lambda>s. P s \<and> \<not> B s\<^bold>}"
+  using H_while[of "\<lceil>P\<rceil>" "\<lceil>B\<rceil>" X]
+  unfolding kat_while_inv_def by auto
+
+\<comment> \<open> Finite Iteration \<close>
 
 abbreviation loopi_sugar :: "'a nd_fun \<Rightarrow> 'a pred \<Rightarrow> 'a nd_fun" ("LOOP _ INV _ " [64,64] 63)
   where "LOOP X INV I \<equiv> kat_loop_inv X \<lceil>I\<rceil>"
 
-lemma H_loop: "Hoare \<lceil>P\<rceil> X \<lceil>P\<rceil> \<Longrightarrow> Hoare \<lceil>P\<rceil> (LOOP X INV I) \<lceil>P\<rceil>"
+lemma H_loop: "\<^bold>{P\<^bold>} X \<^bold>{P\<^bold>} \<Longrightarrow> \<^bold>{P\<^bold>} (LOOP X INV I) \<^bold>{P\<^bold>}"
   by (auto intro: H_loop)
 
-lemma H_loopI: "Hoare \<lceil>I\<rceil> X \<lceil>I\<rceil> \<Longrightarrow> \<lceil>P\<rceil> \<le> \<lceil>I\<rceil> \<Longrightarrow> \<lceil>I\<rceil> \<le> \<lceil>Q\<rceil> \<Longrightarrow> Hoare \<lceil>P\<rceil> (LOOP X INV I) \<lceil>Q\<rceil>"
+lemma H_loopI: "\<^bold>{I\<^bold>} X \<^bold>{I\<^bold>} \<Longrightarrow> \<lceil>P\<rceil> \<le> \<lceil>I\<rceil> \<Longrightarrow> \<lceil>I\<rceil> \<le> \<lceil>Q\<rceil> \<Longrightarrow> \<^bold>{P\<^bold>} (LOOP X INV I) \<^bold>{Q\<^bold>}"
   using H_loop_inv[of "\<lceil>P\<rceil>" "\<lceil>I\<rceil>" X "\<lceil>Q\<rceil>"] by auto
 
 
-subsection\<open> Verification of hybrid programs \<close>
+subsubsection \<open> Evolution commands \<close>
 
 \<comment> \<open>Verification by providing evolution\<close>
 
@@ -218,13 +204,13 @@ definition g_evol :: "(('a::ord) \<Rightarrow> 'b \<Rightarrow> 'b) \<Rightarrow
 
 lemma sH_g_evol[simp]:  
   fixes \<phi> :: "('a::preorder) \<Rightarrow> 'b \<Rightarrow> 'b"
-  shows "Hoare \<lceil>P\<rceil> (EVOL \<phi> G U) \<lceil>Q\<rceil> = (\<forall>s. P s \<longrightarrow> (\<forall>t\<in>U s. (\<forall>\<tau>\<in>down (U s) t. G (\<phi> \<tau> s)) \<longrightarrow> Q (\<phi> t s)))"
+  shows "\<^bold>{P\<^bold>} (EVOL \<phi> G U) \<^bold>{Q\<^bold>} = (\<forall>s. P s \<longrightarrow> (\<forall>t\<in>U s. (\<forall>\<tau>\<in>down (U s) t. G (\<phi> \<tau> s)) \<longrightarrow> Q (\<phi> t s)))"
   unfolding ndfun_kat_H g_evol_def g_orbit_eq by auto
 
 lemma H_g_evol: 
   fixes \<phi> :: "('a::preorder) \<Rightarrow> 'b \<Rightarrow> 'b"
   assumes "P = (\<lambda>s. (\<forall>t\<in>U s. (\<forall>\<tau>\<in>down (U s) t. G (\<phi> \<tau> s)) \<longrightarrow> Q (\<phi> t s)))"
-  shows "Hoare \<lceil>P\<rceil> (EVOL \<phi> G U) \<lceil>Q\<rceil>"
+  shows "\<^bold>{P\<^bold>} (EVOL \<phi> G U) \<^bold>{Q\<^bold>}"
   by (simp add: assms)
 
 \<comment> \<open>Verification by providing solutions\<close>
@@ -235,10 +221,10 @@ definition g_ode ::"(real \<Rightarrow> ('a::banach)\<Rightarrow>'a) \<Rightarro
 
 lemma H_g_orbital: 
   "P = (\<lambda>s. (\<forall>X\<in>ivp_sols f U S t\<^sub>0 s. \<forall>t\<in>U s. (\<forall>\<tau>\<in>down (U s) t. G (X \<tau>)) \<longrightarrow> Q (X t))) \<Longrightarrow> 
-  Hoare \<lceil>P\<rceil> (x\<acute>= f & G on U S @ t\<^sub>0) \<lceil>Q\<rceil>"
+  \<^bold>{P\<^bold>} (x\<acute>= f & G on U S @ t\<^sub>0) \<^bold>{Q\<^bold>}"
   unfolding ndfun_kat_H g_ode_def g_orbital_eq by clarsimp
 
-lemma sH_g_orbital: "Hoare \<lceil>P\<rceil> (x\<acute>= f & G on U S @ t\<^sub>0) \<lceil>Q\<rceil> = 
+lemma sH_g_orbital: "\<^bold>{P\<^bold>} (x\<acute>= f & G on U S @ t\<^sub>0) \<^bold>{Q\<^bold>} = 
   (\<forall>s. P s \<longrightarrow> (\<forall>X\<in>ivp_sols f U S t\<^sub>0 s. \<forall>t\<in>U s. (\<forall>\<tau>\<in>down (U s) t. G (X \<tau>)) \<longrightarrow> Q (X t)))"
   unfolding g_orbital_eq g_ode_def ndfun_kat_H by auto
 
@@ -247,7 +233,7 @@ begin
 
 lemma sH_g_ode_subset: 
   assumes "\<And>s. s \<in> S \<Longrightarrow> 0 \<in> U s \<and> is_interval (U s) \<and> U s \<subseteq> T"
-  shows "Hoare \<lceil>P\<rceil> (x\<acute>= (\<lambda>t. f) & G on U S @ 0) \<lceil>Q\<rceil> = 
+  shows "\<^bold>{P\<^bold>} (x\<acute>= (\<lambda>t. f) & G on U S @ 0) \<^bold>{Q\<^bold>} = 
   (\<forall>s\<in>S. P s \<longrightarrow> (\<forall>t\<in>U s. (\<forall>\<tau>\<in>down (U s) t. G (\<phi> \<tau> s)) \<longrightarrow> Q (\<phi> t s)))"
 proof(unfold sH_g_orbital, clarsimp, safe)
   fix s t
@@ -272,20 +258,20 @@ qed
 lemma H_g_ode_subset:
   assumes "\<And>s. s \<in> S \<Longrightarrow> 0 \<in> U s \<and> is_interval (U s) \<and> U s \<subseteq> T"
     and "P = (\<lambda>s. s \<in> S \<longrightarrow> (\<forall>t\<in>U s. (\<forall>\<tau>\<in>down (U s) t. G (\<phi> \<tau> s)) \<longrightarrow> Q (\<phi> t s)))" 
-  shows "Hoare \<lceil>P\<rceil> (x\<acute>= (\<lambda>t. f) & G on U S @ 0) \<lceil>Q\<rceil>"
+  shows "\<^bold>{P\<^bold>} (x\<acute>= (\<lambda>t. f) & G on U S @ 0) \<^bold>{Q\<^bold>}"
   using assms apply(subst sH_g_ode_subset[OF assms(1)])
   unfolding assms by auto
 
-lemma sH_g_ode: "Hoare \<lceil>P\<rceil> (x\<acute>= (\<lambda>t. f) & G on (\<lambda>s. T) S @ 0) \<lceil>Q\<rceil> = 
+lemma sH_g_ode: "\<^bold>{P\<^bold>} (x\<acute>= (\<lambda>t. f) & G on (\<lambda>s. T) S @ 0) \<^bold>{Q\<^bold>} = 
   (\<forall>s\<in>S. P s \<longrightarrow> (\<forall>t\<in>T. (\<forall>\<tau>\<in>down T t. G (\<phi> \<tau> s)) \<longrightarrow> Q (\<phi> t s)))"
   by (subst sH_g_ode_subset, auto simp: init_time interval_time)
 
-lemma sH_g_ode_ivl: "t \<ge> 0 \<Longrightarrow> t \<in> T \<Longrightarrow> Hoare \<lceil>P\<rceil> (x\<acute>= (\<lambda>t. f) & G on (\<lambda>s. {0..t}) S @ 0) \<lceil>Q\<rceil> = 
+lemma sH_g_ode_ivl: "t \<ge> 0 \<Longrightarrow> t \<in> T \<Longrightarrow> \<^bold>{P\<^bold>} (x\<acute>= (\<lambda>t. f) & G on (\<lambda>s. {0..t}) S @ 0) \<^bold>{Q\<^bold>} = 
   (\<forall>s\<in>S. P s \<longrightarrow> (\<forall>t\<in>{0..t}. (\<forall>\<tau>\<in>{0..t}. G (\<phi> \<tau> s)) \<longrightarrow> Q (\<phi> t s)))"
   apply(subst sH_g_ode_subset; clarsimp, (force)?)
   using init_time interval_time mem_is_interval_1_I by blast
 
-lemma sH_orbit: "Hoare \<lceil>P\<rceil> (\<gamma>\<^sup>\<phi>\<^sup>\<bullet>) \<lceil>Q\<rceil> = (\<forall>s \<in> S. P s \<longrightarrow> (\<forall> t \<in> T. Q (\<phi> t s)))"
+lemma sH_orbit: "\<^bold>{P\<^bold>} \<gamma>\<^sup>\<phi>\<^sup>\<bullet> \<^bold>{Q\<^bold>}  = (\<forall>s \<in> S. P s \<longrightarrow> (\<forall> t \<in> T. Q (\<phi> t s)))"
   using sH_g_ode unfolding orbit_def g_ode_def by auto
 
 end
@@ -298,21 +284,21 @@ definition g_ode_inv :: "(real \<Rightarrow> ('a::banach)\<Rightarrow>'a) \<Righ
 
 lemma sH_g_orbital_guard: 
   assumes "R = (\<lambda>s. G s \<and> Q s)"
-  shows "Hoare \<lceil>P\<rceil> (x\<acute>= f & G on T S @ t\<^sub>0) \<lceil>Q\<rceil> = Hoare \<lceil>P\<rceil> (x\<acute>= f & G on T S @ t\<^sub>0) \<lceil>R\<rceil>" 
+  shows "\<^bold>{P\<^bold>} (x\<acute>= f & G on U S @ t\<^sub>0) \<^bold>{Q\<^bold>} = \<^bold>{P\<^bold>} (x\<acute>= f & G on U S @ t\<^sub>0) \<^bold>{R\<^bold>}" 
   using assms unfolding g_orbital_eq ndfun_kat_H ivp_sols_def g_ode_def by auto
 
 lemma sH_g_orbital_inv:
-  assumes "\<lceil>P\<rceil> \<le> \<lceil>I\<rceil>" and "Hoare \<lceil>I\<rceil> (x\<acute>= f & G on T S @ t\<^sub>0) \<lceil>I\<rceil>" and "\<lceil>I\<rceil> \<le> \<lceil>Q\<rceil>"
-  shows "Hoare \<lceil>P\<rceil> (x\<acute>= f & G on T S @ t\<^sub>0) \<lceil>Q\<rceil>"
+  assumes "\<lceil>P\<rceil> \<le> \<lceil>I\<rceil>" and "\<^bold>{I\<^bold>} (x\<acute>= f & G on U S @ t\<^sub>0) \<^bold>{I\<^bold>}" and "\<lceil>I\<rceil> \<le> \<lceil>Q\<rceil>"
+  shows " \<^bold>{P\<^bold>} (x\<acute>= f & G on U S @ t\<^sub>0) \<^bold>{Q\<^bold>}"
   using assms(1) apply(rule_tac p'="\<lceil>I\<rceil>" in H_consl, simp)
   using assms(3) apply(rule_tac q'="\<lceil>I\<rceil>" in H_consr, simp)
   using assms(2) by simp
 
-lemma sH_diff_inv[simp]: "Hoare \<lceil>I\<rceil> (x\<acute>= f & G on T S @ t\<^sub>0) \<lceil>I\<rceil> = diff_invariant I f T S t\<^sub>0 G"
+lemma sH_diff_inv[simp]: "\<^bold>{I\<^bold>} (x\<acute>= f & G on U S @ t\<^sub>0) \<^bold>{I\<^bold>} = diff_invariant I f U S t\<^sub>0 G"
   unfolding diff_invariant_eq ndfun_kat_H g_orbital_eq g_ode_def by auto
 
-lemma H_g_ode_inv: "Hoare \<lceil>I\<rceil> (x\<acute>= f & G on T S @ t\<^sub>0) \<lceil>I\<rceil> \<Longrightarrow> \<lceil>P\<rceil> \<le> \<lceil>I\<rceil> \<Longrightarrow> 
-  \<lceil>\<lambda>s. I s \<and> G s\<rceil> \<le> \<lceil>Q\<rceil> \<Longrightarrow> Hoare \<lceil>P\<rceil> (x\<acute>= f & G on T S @ t\<^sub>0 DINV I) \<lceil>Q\<rceil>"
+lemma H_g_ode_inv: "\<^bold>{I\<^bold>} (x\<acute>= f & G on U S @ t\<^sub>0) \<^bold>{I\<^bold>} \<Longrightarrow> \<lceil>P\<rceil> \<le> \<lceil>I\<rceil> \<Longrightarrow> 
+  \<lceil>\<lambda>s. I s \<and> G s\<rceil> \<le> \<lceil>Q\<rceil> \<Longrightarrow> \<^bold>{P\<^bold>} (x\<acute>= f & G on U S @ t\<^sub>0 DINV I) \<^bold>{Q\<^bold>}"
   unfolding g_ode_inv_def apply(rule_tac q'="\<lceil>\<lambda>s. I s \<and> G s\<rceil>" in H_consr, simp)
   apply(subst sH_g_orbital_guard[symmetric], force)
   by (rule_tac I="I" in sH_g_orbital_inv, simp_all)
@@ -325,31 +311,50 @@ subsection \<open> Refinement Components \<close>
 lemma R_skip: "(\<forall>s. P s \<longrightarrow> Q s) \<Longrightarrow> 1 \<le> Ref \<lceil>P\<rceil> \<lceil>Q\<rceil>"
   by (auto simp: spec_def ndfun_kat_H one_nd_fun_def)
 
-\<comment> \<open> Composition \<close>
+\<comment> \<open> Abort \<close>
+
+lemma R_abort: "abort \<le> Ref \<lceil>P\<rceil> \<lceil>Q\<rceil>"
+  by (rule R2, simp)
+
+\<comment> \<open> Sequential Composition \<close>
 
 lemma R_seq: "(Ref \<lceil>P\<rceil> \<lceil>R\<rceil>) ; (Ref \<lceil>R\<rceil> \<lceil>Q\<rceil>) \<le> Ref \<lceil>P\<rceil> \<lceil>Q\<rceil>"
   using R_seq by blast
 
-lemma R_seq_rule: "X \<le> Ref \<lceil>P\<rceil> \<lceil>R\<rceil> \<Longrightarrow> Y \<le> Ref \<lceil>R\<rceil> \<lceil>Q\<rceil> \<Longrightarrow> X; Y \<le> Ref \<lceil>P\<rceil> \<lceil>Q\<rceil>"
+lemma R_seq_law: "X \<le> Ref \<lceil>P\<rceil> \<lceil>R\<rceil> \<Longrightarrow> Y \<le> Ref \<lceil>R\<rceil> \<lceil>Q\<rceil> \<Longrightarrow> X; Y \<le> Ref \<lceil>P\<rceil> \<lceil>Q\<rceil>"
   unfolding spec_def by (rule H_seq)
 
 lemmas R_seq_mono = mult_isol_var
+
+\<comment> \<open> Nondeterministic Choice \<close>
+
+lemma R_choice: "(Ref \<lceil>P\<rceil> \<lceil>Q\<rceil>) + (Ref \<lceil>P\<rceil> \<lceil>Q\<rceil>) \<le> Ref \<lceil>P\<rceil> \<lceil>Q\<rceil>"
+  using R_choice[of "\<lceil>P\<rceil>" "\<lceil>Q\<rceil>"] .
+
+lemma R_choice_law: "X \<le> Ref \<lceil>P\<rceil> \<lceil>Q\<rceil> \<Longrightarrow> Y \<le> Ref \<lceil>P\<rceil> \<lceil>Q\<rceil> \<Longrightarrow> X + Y \<le> Ref \<lceil>P\<rceil> \<lceil>Q\<rceil>"
+  using join.le_supI .
+
+lemma R_choice_mono: "P' \<le> P \<Longrightarrow> Q' \<le> Q \<Longrightarrow> P' + Q' \<subseteq> P + Q"
+  using set_plus_mono2 .
 
 \<comment> \<open> Assignment \<close>
 
 lemma R_assign: "(x ::= e) \<le> Ref \<lceil>\<lambda>s. P (\<chi> j. ((($) s)(x := e s)) j)\<rceil> \<lceil>P\<rceil>"
   unfolding spec_def by (rule H_assign, clarsimp simp: fun_eq_iff fun_upd_def)
 
-lemma R_assign_rule: "(\<forall>s. P s \<longrightarrow> Q (\<chi> j. ((($) s)(x := (e s))) j)) \<Longrightarrow> (x ::= e) \<le> Ref \<lceil>P\<rceil> \<lceil>Q\<rceil>"
+lemma R_assign_law: 
+  "(\<forall>s. P s \<longrightarrow> Q (\<chi> j. ((($) s)(x := (e s))) j)) \<Longrightarrow> (x ::= e) \<le> Ref \<lceil>P\<rceil> \<lceil>Q\<rceil>"
   unfolding sH_assign[symmetric] spec_def .
 
-lemma R_assignl: "P = (\<lambda>s. R (\<chi> j. ((($) s)(x := e s)) j)) \<Longrightarrow> (x ::= e) ; Ref \<lceil>R\<rceil> \<lceil>Q\<rceil> \<le> Ref \<lceil>P\<rceil> \<lceil>Q\<rceil>"
-  apply(rule_tac R=R in R_seq_rule)
-  by (rule_tac R_assign_rule, simp_all)
+lemma R_assignl: 
+  "P = (\<lambda>s. R (\<chi> j. ((($) s)(x := e s)) j)) \<Longrightarrow> (x ::= e) ; Ref \<lceil>R\<rceil> \<lceil>Q\<rceil> \<le> Ref \<lceil>P\<rceil> \<lceil>Q\<rceil>"
+  apply(rule_tac R=R in R_seq_law)
+  by (rule_tac R_assign_law, simp_all)
 
-lemma R_assignr: "R = (\<lambda>s. Q (\<chi> j. ((($) s)(x := e s)) j)) \<Longrightarrow> Ref \<lceil>P\<rceil> \<lceil>R\<rceil>; (x ::= e) \<le> Ref \<lceil>P\<rceil> \<lceil>Q\<rceil>"
-  apply(rule_tac R=R in R_seq_rule, simp)
-  by (rule_tac R_assign_rule, simp)
+lemma R_assignr: 
+  "R = (\<lambda>s. Q (\<chi> j. ((($) s)(x := e s)) j)) \<Longrightarrow> Ref \<lceil>P\<rceil> \<lceil>R\<rceil>; (x ::= e) \<le> Ref \<lceil>P\<rceil> \<lceil>Q\<rceil>"
+  apply(rule_tac R=R in R_seq_law, simp)
+  by (rule_tac R_assign_law, simp)
 
 lemma "(x ::= e) ; Ref \<lceil>Q\<rceil> \<lceil>Q\<rceil> \<le> Ref \<lceil>(\<lambda>s. Q (\<chi> j. ((($) s)(x := e s)) j))\<rceil> \<lceil>Q\<rceil>"
   by (rule R_assignl) simp
@@ -357,26 +362,53 @@ lemma "(x ::= e) ; Ref \<lceil>Q\<rceil> \<lceil>Q\<rceil> \<le> Ref \<lceil>(\<
 lemma "Ref \<lceil>Q\<rceil> \<lceil>(\<lambda>s. Q (\<chi> j. ((($) s)(x := e s)) j))\<rceil>; (x ::= e) \<le> Ref \<lceil>Q\<rceil> \<lceil>Q\<rceil>"
   by (rule R_assignr) simp
 
-\<comment> \<open> Conditional \<close>
+\<comment> \<open> Nondeterministic Assignment \<close>
 
-lemma R_cond: "(IF B THEN Ref \<lceil>\<lambda>s. B s \<and> P s\<rceil> \<lceil>Q\<rceil> ELSE Ref \<lceil>\<lambda>s. \<not> B s \<and> P s\<rceil> \<lceil>Q\<rceil>) \<le> Ref \<lceil>P\<rceil> \<lceil>Q\<rceil>"
+lemma R_nondet_assign: "(x ::= ?) \<le> Ref \<lceil>\<lambda>s. \<forall>k. P (\<chi> j. ((($) s)(x := k)) j)\<rceil> \<lceil>P\<rceil>"
+  unfolding spec_def by (rule H_nondet_assign)
+
+lemma R_nondet_assign_law: 
+  "(\<forall>s. P s \<longrightarrow> (\<forall>k. Q (\<chi> j. ((($) s)(x := k)) j))) \<Longrightarrow> (x ::= ?) \<le> Ref \<lceil>P\<rceil> \<lceil>Q\<rceil>"
+  unfolding sH_nondet_assign[symmetric] by (rule R2)
+
+\<comment> \<open> Conditional Statement \<close>
+
+lemma R_cond: 
+  "(IF B THEN Ref \<lceil>\<lambda>s. B s \<and> P s\<rceil> \<lceil>Q\<rceil> ELSE Ref \<lceil>\<lambda>s. \<not> B s \<and> P s\<rceil> \<lceil>Q\<rceil>) \<le> Ref \<lceil>P\<rceil> \<lceil>Q\<rceil>"
   using R_cond[of "\<lceil>B\<rceil>" "\<lceil>P\<rceil>" "\<lceil>Q\<rceil>"] by simp
 
 lemma R_cond_mono: "X \<le> X' \<Longrightarrow> Y \<le> Y' \<Longrightarrow> (IF P THEN X ELSE Y) \<le> IF P THEN X' ELSE Y'"
   unfolding kat_cond_def times_nd_fun_def plus_nd_fun_def n_op_nd_fun_def
   by (auto simp: kcomp_def less_eq_nd_fun_def p2ndf_def le_fun_def)
 
+lemma R_cond_law: "X \<le> Ref \<lceil>\<lambda>s. B s \<and> P s\<rceil> \<lceil>Q\<rceil> \<Longrightarrow> Y \<le> Ref \<lceil>\<lambda>s. \<not> B s \<and> P s\<rceil> \<lceil>Q\<rceil> \<Longrightarrow> 
+  (IF B THEN X ELSE Y) \<le> Ref \<lceil>P\<rceil> \<lceil>Q\<rceil>"
+  by (rule order_trans; (rule R_cond_mono)?, (rule R_cond)?) auto
+
 \<comment> \<open> While loop \<close>
 
-lemma R_while: "WHILE Q INV I DO (Ref \<lceil>\<lambda>s. P s \<and> Q s\<rceil> \<lceil>P\<rceil>) \<le> Ref \<lceil>P\<rceil> \<lceil>\<lambda>s. P s \<and> \<not> Q s\<rceil>"
-  unfolding kat_while_inv_def using R_while[of "\<lceil>Q\<rceil>" "\<lceil>P\<rceil>"] by simp
+lemma R_while: "K = (\<lambda>s. P s \<and> \<not> B s) \<Longrightarrow>
+  WHILE B INV I DO (Ref \<lceil>\<lambda>s. P s \<and> B s\<rceil> \<lceil>P\<rceil>) \<le> Ref \<lceil>P\<rceil> \<lceil>K\<rceil>"
+  unfolding kat_while_inv_def using R_while[of "\<lceil>B\<rceil>" "\<lceil>P\<rceil>"] by simp
+
+lemma R_whileI:
+  "X \<le> Ref \<lceil>I\<rceil> \<lceil>I\<rceil> \<Longrightarrow> \<lceil>P\<rceil> \<le> \<lceil>\<lambda>s. I s \<and> B s\<rceil> \<Longrightarrow> \<lceil>\<lambda>s. I s \<and> \<not> B s\<rceil> \<le> \<lceil>Q\<rceil> \<Longrightarrow> 
+  WHILE B INV I DO X \<le> Ref \<lceil>P\<rceil> \<lceil>Q\<rceil>"
+  by (rule R2, rule H_while_inv, auto simp: ndfun_kat_H spec_def)
 
 lemma R_while_mono: "X \<le> X' \<Longrightarrow> (WHILE P INV I DO X) \<le> WHILE P INV I DO X'"
   by (simp add: kat_while_inv_def kat_while_def mult_isol mult_isor star_iso)
 
-\<comment> \<open> Finite loop \<close>
+lemma R_while_law: "X \<le> Ref \<lceil>\<lambda>s. P s \<and> B s\<rceil> \<lceil>P\<rceil> \<Longrightarrow> Q = (\<lambda>s. P s \<and> \<not> B s) \<Longrightarrow> 
+  (WHILE B INV I DO X) \<le> Ref \<lceil>P\<rceil> \<lceil>Q\<rceil>"
+  by (rule order_trans; (rule R_while_mono)?, (rule R_while)?)
+
+\<comment> \<open> Finite Iteration \<close>
 
 lemma R_loop: "X \<le> Ref \<lceil>I\<rceil> \<lceil>I\<rceil> \<Longrightarrow> \<lceil>P\<rceil> \<le> \<lceil>I\<rceil> \<Longrightarrow> \<lceil>I\<rceil> \<le> \<lceil>Q\<rceil> \<Longrightarrow> LOOP X INV I \<le> Ref \<lceil>P\<rceil> \<lceil>Q\<rceil>"
+  unfolding spec_def using H_loopI by blast
+
+lemma R_loopI: "X \<le> Ref \<lceil>I\<rceil> \<lceil>I\<rceil> \<Longrightarrow> \<lceil>P\<rceil> \<le> \<lceil>I\<rceil> \<Longrightarrow> \<lceil>I\<rceil> \<le> \<lceil>Q\<rceil> \<Longrightarrow> LOOP X INV I \<le> Ref \<lceil>P\<rceil> \<lceil>Q\<rceil>"
   unfolding spec_def using H_loopI by blast
 
 lemma R_loop_mono: "X \<le> X' \<Longrightarrow> LOOP X INV I \<le> LOOP X' INV I"
@@ -389,28 +421,30 @@ lemma R_g_evol:
   shows "(EVOL \<phi> G U) \<le> Ref \<lceil>\<lambda>s. \<forall>t\<in>U s. (\<forall>\<tau>\<in>down (U s) t. G (\<phi> \<tau> s)) \<longrightarrow> P (\<phi> t s)\<rceil> \<lceil>P\<rceil>"
   unfolding spec_def by (rule H_g_evol, simp)
 
-lemma R_g_evol_rule: 
+lemma R_g_evol_law: 
   fixes \<phi> :: "('a::preorder) \<Rightarrow> 'b \<Rightarrow> 'b"
-  shows "(\<forall>s. P s \<longrightarrow> (\<forall>t\<in>U s. (\<forall>\<tau>\<in>down (U s) t. G (\<phi> \<tau> s)) \<longrightarrow> Q (\<phi> t s))) \<Longrightarrow> (EVOL \<phi> G U) \<le> Ref \<lceil>P\<rceil> \<lceil>Q\<rceil>"
+  shows "(\<forall>s. P s \<longrightarrow> (\<forall>t\<in>U s. (\<forall>\<tau>\<in>down (U s) t. G (\<phi> \<tau> s)) \<longrightarrow> Q (\<phi> t s))) \<Longrightarrow> 
+  (EVOL \<phi> G U) \<le> Ref \<lceil>P\<rceil> \<lceil>Q\<rceil>"
   unfolding sH_g_evol[symmetric] spec_def .
 
 lemma R_g_evoll: 
   fixes \<phi> :: "('a::preorder) \<Rightarrow> 'b \<Rightarrow> 'b"
   shows "P = (\<lambda>s. \<forall>t\<in>U s. (\<forall>\<tau>\<in>down (U s) t. G (\<phi> \<tau> s)) \<longrightarrow> R (\<phi> t s)) \<Longrightarrow> 
   (EVOL \<phi> G U) ; Ref \<lceil>R\<rceil> \<lceil>Q\<rceil> \<le> Ref \<lceil>P\<rceil> \<lceil>Q\<rceil>"
-  apply(rule_tac R=R in R_seq_rule)
-  by (rule_tac R_g_evol_rule, simp_all)
+  apply(rule_tac R=R in R_seq_law)
+  by (rule_tac R_g_evol_law, simp_all)
 
 lemma R_g_evolr: 
   fixes \<phi> :: "('a::preorder) \<Rightarrow> 'b \<Rightarrow> 'b"
   shows "R = (\<lambda>s. \<forall>t\<in>U s. (\<forall>\<tau>\<in>down (U s) t. G (\<phi> \<tau> s)) \<longrightarrow> Q (\<phi> t s)) \<Longrightarrow> 
   Ref \<lceil>P\<rceil> \<lceil>R\<rceil>; (EVOL \<phi> G U) \<le> Ref \<lceil>P\<rceil> \<lceil>Q\<rceil>"
-  apply(rule_tac R=R in R_seq_rule, simp)
-  by (rule_tac R_g_evol_rule, simp)
+  apply(rule_tac R=R in R_seq_law, simp)
+  by (rule_tac R_g_evol_law, simp)
 
 lemma 
   fixes \<phi> :: "('a::preorder) \<Rightarrow> 'b \<Rightarrow> 'b"
-  shows "EVOL \<phi> G U ; Ref \<lceil>Q\<rceil> \<lceil>Q\<rceil> \<le> Ref \<lceil>\<lambda>s. \<forall>t\<in>U s. (\<forall>\<tau>\<in>down (U s) t. G (\<phi> \<tau> s)) \<longrightarrow> Q (\<phi> t s)\<rceil> \<lceil>Q\<rceil>"
+  shows "EVOL \<phi> G U ; Ref \<lceil>Q\<rceil> \<lceil>Q\<rceil> \<le> 
+  Ref \<lceil>\<lambda>s. \<forall>t\<in>U s. (\<forall>\<tau>\<in>down (U s) t. G (\<phi> \<tau> s)) \<longrightarrow> Q (\<phi> t s)\<rceil> \<lceil>Q\<rceil>"
   by (rule R_g_evoll) simp
 
 lemma 
@@ -425,7 +459,8 @@ begin
 
 lemma R_g_ode_subset: 
   assumes "\<And>s. s \<in> S \<Longrightarrow> 0 \<in> U s \<and> is_interval (U s) \<and> U s \<subseteq> T"
-  shows "(x\<acute>= (\<lambda>t. f) & G on U S @ 0) \<le> Ref \<lceil>\<lambda>s. s\<in>S \<longrightarrow> (\<forall>t\<in>U s. (\<forall>\<tau>\<in>down (U s) t. G (\<phi> \<tau> s)) \<longrightarrow> P (\<phi> t s))\<rceil> \<lceil>P\<rceil>"
+  shows "(x\<acute>= (\<lambda>t. f) & G on U S @ 0) \<le> 
+  Ref \<lceil>\<lambda>s. s\<in>S \<longrightarrow> (\<forall>t\<in>U s. (\<forall>\<tau>\<in>down (U s) t. G (\<phi> \<tau> s)) \<longrightarrow> P (\<phi> t s))\<rceil> \<lceil>P\<rceil>"
   unfolding spec_def by (rule H_g_ode_subset[OF assms], auto)
 
 lemma R_g_ode_rule_subset: 
@@ -438,20 +473,21 @@ lemma R_g_odel_subset:
   assumes "\<And>s. s \<in> S \<Longrightarrow> 0 \<in> U s \<and> is_interval (U s) \<and> U s \<subseteq> T"
     and "P = (\<lambda>s. \<forall>t\<in>U s. (\<forall>\<tau>\<in>down (U s) t. G (\<phi> \<tau> s)) \<longrightarrow> R (\<phi> t s))"
   shows "(x\<acute>= (\<lambda>t. f) & G on U S @ 0) ; Ref \<lceil>R\<rceil> \<lceil>Q\<rceil> \<le> Ref \<lceil>P\<rceil> \<lceil>Q\<rceil>"
-  apply (rule_tac R=R in R_seq_rule, rule_tac R_g_ode_rule_subset)
+  apply (rule_tac R=R in R_seq_law, rule_tac R_g_ode_rule_subset)
   by (simp_all add: assms)
 
 lemma R_g_oder_subset: 
   assumes "\<And>s. s \<in> S \<Longrightarrow> 0 \<in> U s \<and> is_interval (U s) \<and> U s \<subseteq> T"
     and "R = (\<lambda>s. \<forall>t\<in>U s. (\<forall>\<tau>\<in>down (U s) t. G (\<phi> \<tau> s)) \<longrightarrow> Q (\<phi> t s))"
   shows "Ref \<lceil>P\<rceil> \<lceil>R\<rceil>; (x\<acute>= (\<lambda>t. f) & G on U S @ 0) \<le> Ref \<lceil>P\<rceil> \<lceil>Q\<rceil>"
-  apply (rule_tac R=R in R_seq_rule, simp)
+  apply (rule_tac R=R in R_seq_law, simp)
   by (rule_tac R_g_ode_rule_subset, simp_all add: assms)
 
-lemma R_g_ode: "(x\<acute>= (\<lambda>t. f) & G on (\<lambda>s. T) S @ 0) \<le> Ref \<lceil>\<lambda>s. s\<in>S \<longrightarrow> (\<forall>t\<in>T. (\<forall>\<tau>\<in>down T t. G (\<phi> \<tau> s)) \<longrightarrow> P (\<phi> t s))\<rceil> \<lceil>P\<rceil>"
+lemma R_g_ode: "(x\<acute>= (\<lambda>t. f) & G on (\<lambda>s. T) S @ 0) \<le> 
+  Ref \<lceil>\<lambda>s. s\<in>S \<longrightarrow> (\<forall>t\<in>T. (\<forall>\<tau>\<in>down T t. G (\<phi> \<tau> s)) \<longrightarrow> P (\<phi> t s))\<rceil> \<lceil>P\<rceil>"
   by (rule R_g_ode_subset, auto simp: init_time interval_time)
 
-lemma R_g_ode_rule: "(\<forall>s\<in>S. P s \<longrightarrow> (\<forall>t\<in>T. (\<forall>\<tau>\<in>down T t. G (\<phi> \<tau> s)) \<longrightarrow> Q (\<phi> t s))) \<Longrightarrow> 
+lemma R_g_ode_law: "(\<forall>s\<in>S. P s \<longrightarrow> (\<forall>t\<in>T. (\<forall>\<tau>\<in>down T t. G (\<phi> \<tau> s)) \<longrightarrow> Q (\<phi> t s))) \<Longrightarrow> 
   (x\<acute>= (\<lambda>t. f) & G on (\<lambda>s. T) S @ 0) \<le> Ref \<lceil>P\<rceil> \<lceil>Q\<rceil>"
   unfolding sH_g_ode[symmetric] by (rule R2)
 
@@ -479,7 +515,8 @@ lemma R_g_ode_inv: "diff_invariant I f T S t\<^sub>0 G \<Longrightarrow> \<lceil
 
 subsection \<open> Derivation of the rules of dL \<close>
 
-text \<open> We derive a generalised version of some domain specific rules of differential dynamic logic (dL).\<close>
+text \<open> We derive rules of differential dynamic logic (dL). This allows the components to reason 
+in the style of that logic. \<close>
 
 abbreviation g_dl_ode ::"(('a::banach)\<Rightarrow>'a) \<Rightarrow> 'a pred \<Rightarrow> 'a nd_fun" ("(1x\<acute>=_ & _)") 
   where "(x\<acute>=f & G) \<equiv> (x\<acute>= (\<lambda>t. f) & G on (\<lambda>s. {t. t \<ge> 0}) UNIV @ 0)"
@@ -490,25 +527,25 @@ abbreviation g_dl_ode_inv :: "(('a::banach)\<Rightarrow>'a) \<Rightarrow> 'a pre
 lemma diff_solve_rule1:
   assumes "local_flow f UNIV UNIV \<phi>"
     and "\<forall>s. P s \<longrightarrow> (\<forall>t\<ge>0. (\<forall>\<tau>\<in>{0..t}. G (\<phi> \<tau> s)) \<longrightarrow> Q (\<phi> t s))"
-  shows "Hoare \<lceil>P\<rceil> (x\<acute>= f & G) \<lceil>Q\<rceil>"
+  shows "\<^bold>{P\<^bold>} (x\<acute>= f & G) \<^bold>{Q\<^bold>}"
   using assms by(subst local_flow.sH_g_ode_subset, auto)
 
 lemma diff_solve_rule2: 
   fixes c::"'a::{heine_borel, banach}"
   assumes "\<forall>s. P s \<longrightarrow> (\<forall>t\<ge>0. (\<forall>\<tau>\<in>{0..t}. G (s + \<tau> *\<^sub>R c)) \<longrightarrow> Q (s + t *\<^sub>R c))"
-  shows "Hoare \<lceil>P\<rceil> (x\<acute>=(\<lambda>s. c) & G) \<lceil>Q\<rceil>"
+  shows "\<^bold>{P\<^bold>} (x\<acute>=(\<lambda>s. c) & G) \<^bold>{Q\<^bold>}"
   apply(subst local_flow.sH_g_ode_subset[where T=UNIV and \<phi>="(\<lambda> t x. x + t *\<^sub>R c)"])
   using line_is_local_flow assms by auto
 
 lemma diff_weak_rule: 
   assumes "\<lceil>G\<rceil> \<le> \<lceil>Q\<rceil>"
-  shows "Hoare \<lceil>P\<rceil> (x\<acute>= f & G on T S @ t\<^sub>0) \<lceil>Q\<rceil>"
+  shows "\<^bold>{P\<^bold>} (x\<acute>= f & G on U S @ t\<^sub>0) \<^bold>{Q\<^bold>}"
   using assms unfolding g_orbital_eq ndfun_kat_H ivp_sols_def g_ode_def by auto
 
 lemma diff_cut_rule:
   assumes wp_C:"Hoare \<lceil>P\<rceil> (x\<acute>= f & G on U S @ t\<^sub>0) \<lceil>C\<rceil>"
     and wp_Q:"Hoare \<lceil>P\<rceil> (x\<acute>= f & (\<lambda> s. G s \<and> C s) on U S @ t\<^sub>0) \<lceil>Q\<rceil>"
-  shows "Hoare \<lceil>P\<rceil> (x\<acute>= f & G on U S @ t\<^sub>0) \<lceil>Q\<rceil>"
+  shows "\<^bold>{P\<^bold>} (x\<acute>= f & G on U S @ t\<^sub>0) \<^bold>{Q\<^bold>}"
 proof(subst ndfun_kat_H, simp add: g_orbital_eq p2ndf_def g_ode_def, clarsimp)
   fix t::real and X::"real \<Rightarrow> 'a" and s
   assume "P s" and "t \<in> U s"
@@ -526,7 +563,7 @@ qed
 
 lemma diff_inv_rule:
   assumes "\<lceil>P\<rceil> \<le> \<lceil>I\<rceil>" and "diff_invariant I f U S t\<^sub>0 G" and "\<lceil>I\<rceil> \<le> \<lceil>Q\<rceil>"
-  shows "Hoare \<lceil>P\<rceil> (x\<acute>= f & G on U S @ t\<^sub>0) \<lceil>Q\<rceil>"
+  shows "\<^bold>{P\<^bold>} (x\<acute>= f & G on U S @ t\<^sub>0) \<^bold>{Q\<^bold>}"
   apply(subst g_ode_inv_def[symmetric, where I=I], rule H_g_ode_inv)
   unfolding sH_diff_inv using assms by auto
 
