HybridVerifVecs/FVs/AMV_Example.thy
@@ -1,0 +1,184 @@
+(*  Title:       Examples of hybrid systems verifications
+    Author:      Jonathan Julián Huerta y Munive, 2019
+    Maintainer:  Jonathan Julián Huerta y Munive <jjhuertaymunive1@sheffield.ac.uk>
+*)
+
+subsection \<open> AMV verification \<close>
+
+text \<open> We prove partial correctness specifications of some hybrid systems with our
+verification components.\<close>
+
+theory AMV_Example
+  imports 
+    "../HS_VC_Spartan" 
+    Triangle.Angles
+
+begin
+
+
+subsubsection \<open> Type of variables \<close>
+
+(* continuous variables *)
+abbreviation "amv_cstrs \<equiv> {''x'', ''y'', ''vx'', ''vy'', ''ax'', ''ay'', 
+  ''phi'', ''speed'', ''t''}"
+
+(* discrete variables *)
+abbreviation "amv_dstrs \<equiv> {''sSP'', ''hSP'', ''fx'', ''fy'', ''mode''}"
+
+(* all variables *)
+abbreviation "amv_strs \<equiv> {''x'', ''y'', ''vx'', ''vy'', ''ax'', ''ay'', 
+  ''phi'', ''speed'', ''t'', ''sSP'', ''hSP'', ''fx'', ''fy'', ''mode''}"
+
+(* type of variables *)
+typedef AMV = amv_strs
+  morphisms to_str to_var
+  by blast
+
+notation to_var ("\<downharpoonright>\<^sub>V")
+
+abbreviation "amv_terms \<equiv> {\<downharpoonright>\<^sub>V''x'', \<downharpoonright>\<^sub>V''y'', \<downharpoonright>\<^sub>V''vx'', \<downharpoonright>\<^sub>V''vy'', \<downharpoonright>\<^sub>V''ax'', \<downharpoonright>\<^sub>V''ay'', 
+  \<downharpoonright>\<^sub>V''phi'', \<downharpoonright>\<^sub>V''speed'', \<downharpoonright>\<^sub>V''t'', \<downharpoonright>\<^sub>V''sSP'', \<downharpoonright>\<^sub>V''hSP'', \<downharpoonright>\<^sub>V''fx'', \<downharpoonright>\<^sub>V''fy'', \<downharpoonright>\<^sub>V''mode''}"
+
+lemma number_of_program_vars: "CARD(AMV) = 14"
+  using type_definition.card type_definition_AMV by fastforce
+
+instance AMV::finite
+  apply(standard, subst bij_betw_finite[of to_str UNIV amv_strs])
+   apply(rule bij_betwI')
+     apply (simp add: to_str_inject)
+  using to_str apply blast
+   apply (metis to_var_inverse UNIV_I)
+  by simp
+
+abbreviation val_AMV :: "real^AMV \<Rightarrow> string \<Rightarrow> real" (infixl "\<restriction>\<^sub>V" 90)
+  where "s\<restriction>\<^sub>Vstring \<equiv> s $ (to_var string)"
+
+lemma AMV_univ: "(UNIV::AMV set) = amv_terms"
+  by auto (metis AMV.to_str AMV.to_str_inverse insertE singletonD) 
+
+lemma AMV_exhaust: "x = \<downharpoonright>\<^sub>V''x'' \<or> x = \<downharpoonright>\<^sub>V''y'' \<or> x = \<downharpoonright>\<^sub>V''vx'' \<or> x = \<downharpoonright>\<^sub>V''vy'' 
+  \<or> x = \<downharpoonright>\<^sub>V''ax'' \<or> x = \<downharpoonright>\<^sub>V''ay'' \<or> x = \<downharpoonright>\<^sub>V''phi'' \<or> x = \<downharpoonright>\<^sub>V''speed'' 
+  \<or> x = \<downharpoonright>\<^sub>V''t'' \<or> x=\<downharpoonright>\<^sub>V''sSP'' \<or> x=\<downharpoonright>\<^sub>V''hSP'' \<or> x=\<downharpoonright>\<^sub>V''fx'' \<or> x=\<downharpoonright>\<^sub>V''fy'' \<or> x=\<downharpoonright>\<^sub>V''mode''"
+  using AMV_univ by auto
+
+lemma AMV_sum:
+  fixes f :: "AMV \<Rightarrow> ('a::banach)"
+  shows "(\<Sum>i\<in>UNIV. f i) = f (\<downharpoonright>\<^sub>V''x'') + f (\<downharpoonright>\<^sub>V''y'') + f (\<downharpoonright>\<^sub>V''vx'') + f (\<downharpoonright>\<^sub>V''vy'') 
+  + f (\<downharpoonright>\<^sub>V''ax'') + f (\<downharpoonright>\<^sub>V''ay'') + f (\<downharpoonright>\<^sub>V''phi'') + f (\<downharpoonright>\<^sub>V''speed'') + f (\<downharpoonright>\<^sub>V''t'')
+  + f (\<downharpoonright>\<^sub>V''sSP'') + f (\<downharpoonright>\<^sub>V''hSP'') + f (\<downharpoonright>\<^sub>V''fx'') + f (\<downharpoonright>\<^sub>V''fy'') + f (\<downharpoonright>\<^sub>V''mode'')"
+  unfolding AMV_univ by (simp add: to_var_inject)
+
+lemma AMV_induct: "P (\<downharpoonright>\<^sub>V''x'') \<Longrightarrow> P (\<downharpoonright>\<^sub>V''y'') \<Longrightarrow> P (\<downharpoonright>\<^sub>V''vx'') \<Longrightarrow> P (\<downharpoonright>\<^sub>V''vy'') 
+  \<Longrightarrow> P (\<downharpoonright>\<^sub>V''ax'') \<Longrightarrow> P (\<downharpoonright>\<^sub>V''ay'') \<Longrightarrow> P (\<downharpoonright>\<^sub>V''phi'') \<Longrightarrow> P (\<downharpoonright>\<^sub>V''speed'') \<Longrightarrow> P (\<downharpoonright>\<^sub>V''t'')
+  \<Longrightarrow> P (\<downharpoonright>\<^sub>V''sSP'') \<Longrightarrow> P (\<downharpoonright>\<^sub>V''hSP'') \<Longrightarrow> P (\<downharpoonright>\<^sub>V''fx'') \<Longrightarrow> P (\<downharpoonright>\<^sub>V''fy'') \<Longrightarrow> P (\<downharpoonright>\<^sub>V''mode'')
+  \<Longrightarrow> \<forall>i. P i"
+  using AMV_exhaust by metis
+
+lemma AMV_eq:
+  "(s1 = s2) \<longleftrightarrow> (s1\<restriction>\<^sub>V''x'' = s2\<restriction>\<^sub>V''x'' \<and> s1\<restriction>\<^sub>V''y'' = s2\<restriction>\<^sub>V''y'' \<and> s1\<restriction>\<^sub>V''vx'' = s2\<restriction>\<^sub>V''vx'' \<and>
+  s1\<restriction>\<^sub>V''vy'' = s2\<restriction>\<^sub>V''vy'' \<and> s1\<restriction>\<^sub>V''ax'' = s2\<restriction>\<^sub>V''ax'' \<and> s1\<restriction>\<^sub>V''ay'' = s2\<restriction>\<^sub>V''ay'' \<and>
+  s1\<restriction>\<^sub>V''phi'' = s2\<restriction>\<^sub>V''phi'' \<and> s1\<restriction>\<^sub>V''speed'' = s2\<restriction>\<^sub>V''speed'' \<and> s1\<restriction>\<^sub>V''t'' = s2\<restriction>\<^sub>V''t'' \<and>
+  s1\<restriction>\<^sub>V''sSP'' = s2\<restriction>\<^sub>V''sSP'' \<and> s1\<restriction>\<^sub>V''hSP'' = s2\<restriction>\<^sub>V''hSP'' \<and> 
+  s1\<restriction>\<^sub>V''fx'' = s2\<restriction>\<^sub>V''fx'' \<and> s1\<restriction>\<^sub>V''fy'' = s2\<restriction>\<^sub>V''fy'' \<and> s1\<restriction>\<^sub>V''mode'' = s2\<restriction>\<^sub>V''mode'')"
+  apply(clarsimp simp: vec_eq_iff, rule iffI, force)
+  by (rule AMV_induct, auto)
+
+subsubsection \<open> Formalisation of continuous dynamics \<close>
+
+(* abbreviation "\<omega> \<equiv> U(arccos((v + a) \<bullet> v / (\<parallel>v + a\<parallel> * \<parallel>v\<parallel>)) \<triangleleft> \<not> \<parallel>v\<parallel> = 0 \<triangleright> 0)" *)
+abbreviation pos :: "real^AMV \<Rightarrow> real^2"
+  where "pos s \<equiv> (\<chi> i. if i=1 then s\<restriction>\<^sub>V''x'' else s\<restriction>\<^sub>V''y'')"
+
+abbreviation vel :: "real^AMV \<Rightarrow> real^2"
+  where "vel s \<equiv> (\<chi> i. if i=1 then s\<restriction>\<^sub>V''vx'' else s\<restriction>\<^sub>V''vy'')"
+
+abbreviation acc :: "real^AMV \<Rightarrow> real^2"
+  where "acc s \<equiv> (\<chi> i. if i=1 then s\<restriction>\<^sub>V''ax'' else s\<restriction>\<^sub>V''ay'')"
+
+abbreviation "omega s \<equiv> (
+  if \<parallel>vel s\<parallel> \<noteq> 0 then 
+    arccos((vel s + acc s) \<bullet> vel s / ((\<parallel>vel s + acc s\<parallel>) * (\<parallel>vel s\<parallel>))) 
+  else 0)"
+
+
+(* [ p \<mapsto>\<^sub>s v
+  , v \<mapsto>\<^sub>s a
+  , a \<mapsto>\<^sub>s 0
+  , \<phi> \<mapsto>\<^sub>s \<omega>
+  , s \<mapsto>\<^sub>s (v \<bullet> a) / s \<triangleleft> \<not> s = 0 \<triangleright> \<parallel>a\<parallel> 
+  , t \<mapsto>\<^sub>s 1 
+  , old \<mapsto>\<^sub>s 0 ] *)
+abbreviation f_amv :: "real^AMV \<Rightarrow> real^AMV" ("f")
+  where "f s \<equiv> (\<chi> i. 
+    if i=\<downharpoonright>\<^sub>V''x'' then s\<restriction>\<^sub>V''vx'' else (
+    if i=\<downharpoonright>\<^sub>V''y'' then s\<restriction>\<^sub>V''vy'' else (
+    if i=\<downharpoonright>\<^sub>V''vx'' then s\<restriction>\<^sub>V''ax'' else (
+    if i=\<downharpoonright>\<^sub>V''vy'' then s\<restriction>\<^sub>V''ay'' else (
+    if i=\<downharpoonright>\<^sub>V''phi'' then omega s else (
+    if i=\<downharpoonright>\<^sub>V''speed'' then (
+      if s\<restriction>\<^sub>V''speed'' \<noteq> 0 then 
+        (vel s \<bullet> acc s) / s\<restriction>\<^sub>V''speed'' 
+      else 
+        \<parallel>acc s\<parallel>) else (
+    if i=\<downharpoonright>\<^sub>V''t'' then 1 else 0)))))))"
+
+(* abbreviation "ax\<^sub>A\<^sub>V \<equiv> U(&\<^bold>c:t < \<epsilon> \<and> 
+    &\<^bold>c:s *\<^sub>R \<^bold>[[sin(&\<^bold>c:\<phi>),cos(&\<^bold>c:\<phi>)]\<^bold>] = &\<^bold>c:v \<and> 
+    0 \<le> &\<^bold>c:s \<and> &\<^bold>c:s \<le> S)" *)
+abbreviation amv_guard :: "real \<Rightarrow> real \<Rightarrow> real^AMV \<Rightarrow> bool" ("G")
+  where "G \<epsilon> S s \<equiv> s\<restriction>\<^sub>V''t'' < \<epsilon> \<and> 
+    s\<restriction>\<^sub>V''speed'' *\<^sub>R (\<chi> i. if i=1 then sin (s\<restriction>\<^sub>V''phi'') else cos (s\<restriction>\<^sub>V''phi'')) = vel s \<and>
+    0 \<le> s\<restriction>\<^sub>V''speed'' \<and> s\<restriction>\<^sub>V''speed'' \<le> S"
+
+(* abbreviation "Dynamics \<equiv> \<^bold>c:t := 0 ;; ODE" *)
+abbreviation "amv_dyn \<epsilon> S  s \<equiv> (\<downharpoonright>\<^sub>V''t'' ::= (\<lambda>s. 0)) ; (x\<acute>= f & (G \<epsilon> S))"
+
+
+subsubsection \<open> Formalisation of discrete control \<close>
+
+locale AMV =
+  fixes \<epsilon> :: real \<comment> \<open> max. time for ODE \<close>
+    and S :: real \<comment> \<open> max. speed of AMV \<close>
+    and H :: real \<comment> \<open> max. speed of AMV \<close>
+    and HCM :: real \<comment> \<open> modes \<close>
+    and MOM :: real
+    and OCM :: real
+    and wp :: "real^2" \<comment> \<open> waypoint's position  \<close>
+    and Obs :: "(real^2) set" \<comment> \<open> set of obstacles \<close>
+  assumes "Obs = {(\<chi> i::2. (1::real))}"
+    and "HCM = 1"
+    and "MOM = 2"
+    and "OCM = 3"
+begin
+
+(* abbreviation "angOfVec \<equiv> vangle \<^bold>[[0::real,100]\<^bold>]"
+   abbreviation "steerToWP \<equiv> rh := angOfVec(nextWP - &\<^bold>c:p)" *)
+abbreviation "steerToWP \<equiv> (\<downharpoonright>\<^sub>V''t'' ::= (\<lambda>s. vangle (\<chi> i. if i=1 then 0 else 100) (wp - pos s)))"
+
+lemma "vector [0,100] = (\<chi> i::2. if i=1 then (0::real) else 100)"
+  apply(simp add: vec_eq_iff vector_def)
+  using exhaust_2 by auto
+
+(* abbreviation 
+  "LRE \<equiv> ((mode = HCM) \<longrightarrow>\<^sub>r rs := 0.1 ;; steerToWP)
+       \<sqinter> ((mode = OCM) \<longrightarrow>\<^sub>r II)
+       \<sqinter> ((mode = MOM) \<longrightarrow>\<^sub>r 
+             rs := 1 ;; 
+             steerToWP ;; 
+             if (\<exists> o. o \<in> obsReg \<and> \<parallel>&\<^bold>c:p - \<guillemotleft>o\<guillemotright>\<parallel> \<le> 7.5) then mode := HCM ;; rs := 0.1 fi
+          )" *)
+abbreviation "LRE s \<equiv> if s\<restriction>\<^sub>V''mode'' = HCM then ((\<downharpoonright>\<^sub>V''sSP'' ::= (\<lambda>s. H)) ; steerToWP) s else {s}"
+
+
+end
+
+
+(* vangle *)
+term vangle
+
+no_notation f_amv ("f")
+        and amv_guard ("G")
+
+
+
+end
