HybridVerifVecs/hs_vc_examples.thy
@@ -1,6 +1,6 @@
 (*  Title:       Examples of hybrid systems verifications
-    Author:      Jonathan Julián Huerta y Munive, 2019
-    Maintainer:  Jonathan Julián Huerta y Munive <jjhuertaymunive1@sheffield.ac.uk>
+    Author:      Jonathan Julián Huerta y Munive, 2020
+    Maintainer:  Jonathan Julián Huerta y Munive <jonjulian23@gmail.com>
 *)
 
 subsection \<open> Examples \<close>
